## WEEK II - Matching Algorithm

>[🏠 MENU - 6CCS3CFL](year3/6ccs3cfl.md)
>
>[⬅️ WEEK I - Introduction to Compiler](year3/6ccs3cfl/w1.md)
>
>[➡️ WEEK III - Automata & Regular Languages](year3/6ccs3cfl/w3.md)
>
>Outlines:
>
>1. Semantics Derivative
>    - Definition to the Equivalence of Regular Expressions
>    - Definition of Semantics Derivative
>2. The Brzozowski Algorithm
>    - Nullable
>    - Idea of the algorithm
>    - Extended Syntax
>    - Proof

### 2.1. Semantics Derivative

##### 2.1.1. Equivalent Regular Expressions

- Basic Grammar (Recap)
  $$
  \begin{array}{lcll}
  r &::= &\textbf{0}				&\text{Nothing} \\
  ~		&| &\textbf{1}				&\text{Empty String} \\
  ~		&| &c				&\text{Character} \\
  ~		&| &r_1 + r_2		&\text{Alternative/Choice} \\
  ~		&| &r_1 \cdot r_2		&\text{Sequence} \\
  ~		&| &r^*			&\text{Repeat with zero or more times} \\
  \end{array}
  $$
  
- Definition
  
  - Two regular expressions $r_1, r_2$ are **equivalent** provided:
    $$
    r_1 \equiv r_2 \overset{def}= L(r_1) = L(r_2)
    $$
  
- Equivalences

  - Concrete Equivalences
    $$
    \begin{array}{lll}
    (a + b) + c &\equiv & a + (b + c) \\
    a + a &\equiv & a \\
    a + b &\equiv & b + a \\
    (a \cdot b) \cdot c &\equiv & a \cdot (b \cdot c) \\
    c \cdot (a + b) &\equiv & (c \cdot a) + (c \cdot b) \\
    a \cdot a &\not\equiv & a \\
    a + (b \cdot c) &\not\equiv & (a + b) \cdot (a + c) \\
    \end{array}
    $$

  - Corner Cases
    $$
    \begin{array}{lll}
    a \cdot \textbf{0} &\not\equiv & a \\
    a + \textbf{1} &\not\equiv & a \\
    \textbf{1} &\equiv & \textbf{0}^* \\
    \textbf{1}^* &\equiv & \textbf{1} \\
    \textbf{0}^* &\not\equiv & \textbf{0}
    \end{array}
    $$

  - Simplification Rules
    $$
    \begin{array}{lll}
    r + \textbf{0} &\equiv &r \\
    \textbf{0} + r &\equiv &r \\
    r \cdot \textbf{1} &\equiv &r \\
    \textbf{1} \cdot r &\equiv &r \\
    r \cdot \textbf{0} &\equiv &\textbf{0} \\
    \textbf{0} \cdot r &\equiv &\textbf{0} \\
    r + r &\equiv &r
    \end{array}
    $$
    
    > e.g.
    >
    > $$
    > \begin{array}{lcl}((\textbf{1} \cdot b) + \textbf{0}) \cdot r &\implies &((1 \cdot b) + \textbf{0}) \cdot r \\ 
    > ~ &= & (b + \textbf{0}) \cdot r \\ 
    > ~ & = & b \cdot r \end{array}
    > $$
    


##### 2.1.2. Semantic Derivative

- Definition

  - The **Semantic Derivative** of a language take a regular expression $r$, and a character $c$, as arguments and retunrs a new regular expressions. 
  - Essentially this function does: if $r$ can match a string of the form $c::s$, check if the expression can match the rest part of the string $s$ apart from $c$. 
  - This is defined as follows, 
    $$
    \text{der } c\ A \overset{def}= \{s | c :: s \in A \}
    $$
    >  e.g.
    >
    > For $A = \{\text{foo, bar ,frak}\}$ then
    >
    > $\text{der } \text{f } A \overset{def}= \text{\{oo, rak\}}$
    >
    > $\text{der } \text{b } A \overset{def}= \text{\{ar\}}$
    >
    > $\text{der } \text{a } A \overset{def}= \text{\{\}}$

    We can extend this definition to strings
    $$
    \text{der } s\ A \overset{def}= \{s' | s @ s' \in A \}
    $$

  - We could conclude the following property
    $$
    L(\text{der }c \ r) = \text{der }c\ L(r))
    $$

- Recursive Definition
  $$
  \begin{array}{lll}
  \text{der } c\ (\textbf{0}) &\overset{def}= &\textbf{0} \\
  \text{der } c\ (\textbf{1}) &\overset{def}= &\textbf{0} \\
  \text{der } c\ (d) &\overset{def}= &\text{if } c = d \text{ then } \textbf{1} \text{ else } \textbf{0}\\
  \text{der } c\ (r_1 + r_2) &\overset{def}= &\text{der } c\ (r_1) + \text{der } c\ (r_2) \\
  \text{der } c\ (r_1 \cdot r_2) &\overset{def}= &\text{if } \text{nullable}(r_1)\\
  ~ &~ & \text{then } \text{der } c\ (r_1) + r_2 \\
  ~ &~ & \text{else } \text{der } c\ (r_1) \cdot r_2 \\
  \text{der } c\ (r^*) &\overset{def}= & (\text{der } c\ r) \cdot r^* \\
  \text{der } []\ r &\overset{def}= & r \\
  \text{der } (c::s)\ r &\overset{def}= & \text{der } s\ (\text{der } c\ r)
  \end{array}
  $$
  > e.g.
  >
  > Given $r \overset{def}= ((a \cdot b) + c)^*$, we could get that
  >
  > $$
  > \begin{array}{lcl}
  > \text{der } a\ ((a \cdot b) + b)^* &\implies & \text{der } a\ ((a \cdot b) + b)^*\\
  > ~ &= &(\text{der } a\ ((a \cdot b) + b)) \cdot r\\
  > ~ &= &((\text{der } a\ (a \cdot b)) + (\text{der } a\ b)) \cdot r\\
  > ~ &= &((\text{der } a\ a) \cdot b) + (\text{der } a\ b)) \cdot r\\
  > ~ &= &((\textbf{1} \cdot b) + (\text{der } a\ b)) \cdot r\\
  > ~ &= &((\textbf{1} \cdot b) + \textbf{0}) \cdot r\\
  > \end{array}
  > $$
  
- Example

  > e.g. 
  >
  > Does $r_1$ match $abc$?
  >
  > 1. build derivative of $a, r_1$
  > 2. build derivative of $b, r_2$
  > 3. build derivative of $c, r_3$
  > 4. the string is exhausted $(\text{nullable}(r_4))$
  >    test whether $r_4$ can recognise the empty string. 
  > 5. output the result of the rest: $\text{true, false}$

- The Specification for Matching
  - A regular expression $r$ matches a string $s$ provided:
    $$
    s \in L(r)
    $$
  - The point is to decide this problem **as fast as possible**. 

---

### 2.2. The Brzozowski Algorithm

##### 2.2.1.  Nullable

- Definition
  - The algorithm contains two parts. 
  - One is the function $\text{nullable}$, which takes a regular rexpressions as an argument and returns whether it can match the empty string (Boolean in Scala). 
  - Another is for the calculation of dervative. 
  - This is defined recursively as follows: 
    $$
    \begin{array}{lll}
    \text{nullable}(\textbf{0}) &\overset{def}= &\text{false} \\
    \text{nullable}(\textbf{1}) &\overset{def}= &\text{true} \\
    \text{nullable}(c) &\overset{def}= &\text{false} \\
    \text{nullable}(r_1 + r_2) &\overset{def}= &\text{nullable}(r_1) \vee \text{nullable}(r_2) \\
    \text{nullable}(r_1 \cdot r_2) &\overset{def}= &\text{nullable}(r_1) \wedge \text{nullable}(r_2) \\
    \text{nullable}(r^*) &\overset{def}= &\text{true}
    \end{array}
    $$
  
  - The idea behind the function is the following property holds:
    $$
    \text{nullable}(r) \text{ if and only if } [] \in L(r
    $$

##### 2.2.2. The Idea of the Algorithm

- If we want to recognise the string $abc$ with regular expression $r_1$ then

  1. $\text{der }a\ (L(r_1))$
  2. $\text{der } b\ (\text{der } a\ (L(r_1)))$
  3. $\text{der } c\ (\text{der } b\ (\text{der } a\ (L(r_1))))$
  4. Get the result whether the empty string is in this set; same for $\text{der }abc\ (L(r_1))$
     The matching algorithm works similarly, just over regular expressions instead of sets. 
  
- The algorithm using $\text{der}$ and $\text{nullable}$ samilairly. 

  - The function iterates $\text{der}$ takking one character at the time from original string until the string is hausted. 
    $$
    \begin{array}{lll}
    \text{der } []\ r &\overset{def}= & r \\
    \text{der } (c::s)\ r &\overset{def}= & \text{der } s\ (\text{der } c\ r)
    \end{array}
    $$

  - By having the derivative function, we can defined the matcher as follows:
    $$
    \text{matcher }r \ s \overset{def}= \text{nullable}(\text{der } s\ r)
    $$
    We can claim that
    $$
    \text{matcher }r \ s \text{ if and only if } s \in L(r)
    $$

##### 2.2.3. Extended Syntax

- The n-time representation

  - We represented the n-times $a^{\{n\}}$ as a sequence regular expression:
    0: $1$
    1: $a$
    2: $a \cdot a$
    ...
    20: $a \cdot a \cdot ... \cdot a$
  - The time complexity is getting increasing, i.e., this problem is aggravated with $a^?$ being represented as $a + 1$.
  - Solution
    - Extend our regular expressions with explicit constructors
      $$
      \begin{array}{ccl}
      r &::= &... \\
      ~ &| &r^{\{n\}} \\
      ~ &| &r^?
      \end{array}
      $$

    - Definition

      > e.g.
      >
      > Case $n = 2$ and $r \cdot r$
      > $$
      > \begin{array}{lcl}
      > \text{der }c\ (r \cdot r) &\overset{def}= &\text{if nullable}(r) \\
      > ~ &~ &\text{then } (\text{der }c\ r) \cdot r + \text{der }c\ r \\
      > ~ &~ &\text{else } (\text{der }c\ r) \cdot \\
      > ~ &\equiv &(\text{der }c\ r) \cdot r
      > \end{array}
      > $$
      > Proof.

- Negation of Regular Expression

  - Rules
    $\sim r$, represents everything that $r$ cannot recognise
    $L (\sim r) \overset{def}= \text{UNIV} - L(r)$
    $\text{nullable}(\sim r) \overset{def}= \text{not (nullable} (r))$
    $\text{Der }c\ (\sim r) \overset{def}= (\text{Der } c\ r)$
  	
  - Used often for recognising comments, for instance

    `/·∗·(∼ ([a-z]∗ ·∗·/·[a-z]∗))·∗·/`

- The Specification for Matching

  - A regular expression $r$ matches a string $s$ provided:

    $\forall r\ s. \text{ matcher }s\ r $ if and only if $s \in L(r)$

  - The central properties

    $\forall r.\ \text{nullable}(r)$ if and only if $[] \in L(r)$

    $\forall r\ c. L(\text{Der }c\ r) = \text{Der }c\ (L(r))$

##### 2.2.4. Proof about Rexps

- Remember their inductive definition
  - If we want to prove something, say a property $P(r)$, for all regular expressions $r$ then...
- General Process
  - $P$ holds for $\textbf{0}, \textbf{1}, c$
  - $P$ holds for $r_1 + r_2$ under the assumption that $P$ already holds for $r_1, r_2$
  - $P$ holds for $r_1 \cdot r_2$ under the assumption that $P$ already holds for $r_1, r_2$
  - $P$ holds for $r^*$ under the assumption that $P$ already holds for $r$

